Mt/sample.lean
@@ -1,0 +1,73 @@
+import Mt.Reservation
+import Mt.Task
+import Mt.System
+
+structure State where
+  x : Nat
+  y : Nat
+
+structure Reservation where
+  luft  : Nat
+  min_x : Mt.LowerBound
+
+-- [begin] this block will be provided by a `derive` handler in the future --
+-----------------------------------------------------------------------------
+instance : Add Reservation :=⟨fun ⟨luft, min_x⟩ ⟨luft', min_x'⟩ => ⟨luft + luft', min_x + min_x'⟩⟩
+
+private theorem Reservation.add_rw : ∀ a b : Reservation, a + b = ⟨a.luft + b.luft, a.min_x + b.min_x⟩ :=
+  by intros ; rfl
+
+instance ReservationInstance : Mt.IsReservation Reservation where
+  empty := ⟨Mt.IsReservation.empty, Mt.IsReservation.empty⟩
+  assoc :=by intros ; simp only [Reservation.add_rw, Mt.IsReservation.toIsAssociative.assoc]
+  comm :=by intros ; simp only [Reservation.add_rw, Mt.IsReservation.toIsCommutative.comm]
+  empty_add :=by intros ; simp only [Reservation.add_rw, Mt.IsReservation.empty_add]
+
+-----------------------------------------------------------------------------
+-- [end] --------------------------------------------------------------------
+
+def spec : Mt.Spec :={
+  State
+  Reservation
+  validate := fun ⟨luft, min_x⟩ ⟨x, y⟩ => x ≥ y + luft ∧ x ≥ min_x
+  reservations_can_be_dropped :=by
+    simp only []
+    intro r r' state h
+    constructor
+    . exact calc
+        state.y + r.luft ≤ state.y + (r.luft + r'.luft) :=by simp_arith
+        _                ≤ state.x                      :=h.left
+    . sorry -- TODO
+}
+
+open Mt
+open Mt.TaskM
+
+def thread1 : TaskM spec Unit :=do
+  -- increase x atomically; track luft
+  atomic_read_modify λ r s => ⟨
+    { r with luft :=r.luft + 1 },
+    { s with x :=s.x + 1 }⟩
+  
+  -- increase y atomically; track luft
+  atomic_read_modify λ r s => ⟨
+    { r with luft :=r.luft - 1 },
+    { s with y :=(s.y : Nat) + 1 }⟩
+
+  let _ <- atomic_read λ r s => ⟨s.y, { r with min_x :=s.y }⟩
+  let _ <- atomic_read λ r s => ⟨s.x, r⟩
+
+  -- TODO: assert (px ≥ py)
+
+theorem thread1_valid : thread1.valid_for_reservation' ReservationInstance.empty :=by
+  rw [valid_for_reservation']
+  apply valid_for_reservation_bind _ _ _ λ (r : spec.Reservation) _ => r.luft = 1
+  . -- validate ++x
+    apply valid_for_reservation_rm
+    intro (s : State) (⟨luft, min_x⟩ : Reservation) initial_valid
+    simp only [and_true, spec, IsReservation.empty, Nat.zero_add, Reservation.add_rw]
+    simp only [spec, IsReservation.empty, Reservation.add_rw] at initial_valid
+    constructor
+    . sorry
+    . sorry
+  sorry
